Add coordinator start wp with admits for rpcs

src/program_proof/memkv/memkv_coord_definitions.v
@@ -3,6 +3,17 @@ From Goose.github_com.mit_pdos.gokv Require Import memkv.
 From Perennial.program_proof.lockservice Require Import rpc.
 From Perennial.program_proof.memkv Require Import common_proof memkv_shard_definitions.
 
+Definition uCOORD_ADD: nat :=
+  Eval vm_compute in match COORD_ADD with LitV (LitInt n) => int.nat n | _ => 0 end.
+Definition uCOORD_GET: nat :=
+  Eval vm_compute in match COORD_GET with LitV (LitInt n) => int.nat n | _ => 0 end.
+
+Record memkv_coord_names := {
+ coord_urpc_gn : server_chan_gnames ;
+ coord_kv_gn : gname
+}
+.
+
 Section memkv_global_coord_definitions.
 
 (* TODO: should it be heap_globalG or heapG? *)
@@ -14,8 +25,30 @@ Definition all_are_shard_servers (s:list u64) γkv : iProp Σ :=
               (∃ γ, is_shard_server host γ ∗ ⌜γ.(kv_gn) = γkv⌝)
 .
 
-End memkv_global_coord_definitions.
+Definition is_coord_server_addSpec γkv : RPCSpec :=
+  {| spec_rpcid := uCOORD_ADD;
+     spec_ty := u64;
+     spec_Pre := (λ host reqData, ⌜has_encoding_Uint64 reqData host ⌝ ∗
+                                   ∃ γ, ⌜ γ.(kv_gn) = γkv ⌝ ∗ is_shard_server host γ)%I;
+     spec_Post := (λ host reqData repData, True)%I |}.
 
+Definition has_encoding_shardMapping (data : list u8) (l: list u64) :=
+  has_encoding data (map EncUInt64 l).
+
+Definition is_coord_server_getSpec γkv : RPCSpec :=
+  {| spec_rpcid := uCOORD_GET;
+     spec_ty := unit;
+     spec_Pre := (λ _ reqData, True)%I;
+     spec_Post := (λ _ reqData repData,
+                   ∃ (shardMapping : list u64),
+                     ⌜ has_encoding_shardMapping repData shardMapping ⌝ ∗
+                     all_are_shard_servers shardMapping γkv)%I |}.
+
+Definition is_coord_server (host : u64) γ :=
+  ("#HaddSpec" ∷ has_handler γ.(coord_urpc_gn) host (is_coord_server_addSpec γ.(coord_kv_gn)) ∗
+  "#HgetSpec" ∷ has_handler γ.(coord_urpc_gn) host (is_coord_server_getSpec γ.(coord_kv_gn)))%I.
+
+End memkv_global_coord_definitions.
 
 Section memkv_coord_definitions.
 
@@ -27,5 +60,25 @@ Definition own_ShardClerkSet (s:loc) (γkv:gname) : iProp Σ :=
   "HclsMap" ∷ is_map cls_ptr 1 clsM ∗
   "HclsOwn" ∷ [∗ map] host ↦ cl_ptr ∈ clsM, own_MemKVShardClerk cl_ptr γkv
 .
+
+Definition own_MemKVCoordServer (s : loc) γ : iProp Σ :=
+  ∃ cfg (hostShards_ptr : loc) hostShards (clset : loc) shardMap_sl (shardMapping : list u64),
+  "config" ∷ s ↦[MemKVCoord :: "config"] #cfg ∗
+  "hostShards" ∷ s ↦[MemKVCoord :: "hostShards"] #hostShards_ptr ∗
+  "shardClerks" ∷ s ↦[MemKVCoord :: "shardClerks"] #clset ∗
+  "%Hlen_shardMapping" ∷ ⌜Z.of_nat (length shardMapping) = uNSHARD⌝%Z ∗
+  "%HshardMapping_dom" ∷ ⌜∀ i : u64, int.Z i < int.Z uNSHARD → is_Some (shardMapping !! int.nat i)⌝ ∗
+  "shardMap" ∷ s ↦[MemKVCoord :: "shardMap"] (slice_val shardMap_sl) ∗
+  "HshardMap_sl" ∷ typed_slice.is_slice (V:=u64) shardMap_sl HostName 1 shardMapping ∗
+  "#HshardServers" ∷ all_are_shard_servers shardMapping γ ∗
+  "Hmap" ∷ is_map (V:=u64) hostShards_ptr 1 hostShards ∗
+  "HshardClerksSet" ∷ own_ShardClerkSet clset γ.
+
+Definition is_MemKVCoordServer (s:loc) γ : iProp Σ :=
+  ∃ mu,
+  "#Hmu" ∷ readonly (s ↦[MemKVCoord :: "mu"] mu) ∗
+  "#HmuInv" ∷ is_lock memKVN mu (own_MemKVCoordServer s γ.(coord_kv_gn))
+.
+
 
 End memkv_coord_definitions.
