src/program_proof/memkv/memkv_coord_start_proof.v
@@ -1,0 +1,144 @@
+From Perennial.program_proof Require Import dist_prelude.
+From Goose.github_com.mit_pdos.gokv Require Import memkv.
+From Perennial.program_proof.lockservice Require Import rpc.
+
+From Perennial.program_proof.memkv Require Export memkv_shard_definitions memkv_coord_definitions common_proof.
+
+Section memkv_coord_start_proof.
+
+Context `{!heapG Σ, rpcG Σ ShardReplyC, rpcregG Σ, kvMapG Σ}.
+
+Lemma wp_encodeShardMap s (shardMap_sl : Slice.t) (shardMapping : list u64) :
+  {{{ "Hs_ptr" ∷ s ↦[slice.T HostName] (slice_val shardMap_sl) ∗
+      "HshardMap_sl" ∷ typed_slice.is_slice (V:=u64) shardMap_sl HostName 1 shardMapping
+  }}}
+    encodeShardMap #s
+  {{{ (sl: Slice.t) (data: list u8), RET (slice_val sl);
+      "%Henc" ∷ ⌜ has_encoding_shardMapping data shardMapping ⌝ ∗
+      "Hdata" ∷  typed_slice.is_slice sl byteT 1 data ∗
+      "Hs_ptr" ∷ s ↦[slice.T HostName] (slice_val shardMap_sl) ∗
+      "HshardMap_sl" ∷ typed_slice.is_slice (V:=u64) shardMap_sl HostName 1 shardMapping
+  }}}.
+Proof.
+  wp_pures. iIntros (Φ) "H HΦ".
+  iNamed "H".
+  wp_lam.
+Admitted.
+
+Lemma wp_MemKVCoord__AddServerRPC s x γ γsh rep dummy_rep_sl :
+  {{{ "#His_memkv" ∷ is_MemKVCoordServer s γ ∗
+      "#His_shard" ∷ is_shard_server x γsh ∗
+      "Hrep" ∷ rep ↦[slice.T byteT] dummy_rep_sl
+  }}}
+    MemKVCoord__AddServerRPC #s #x
+  {{{ (rep_sl : Slice.t) (repData : list u8), RET #();
+     rep ↦[slice.T byteT] (slice_val rep_sl) ∗
+     typed_slice.is_slice rep_sl byteT 1 repData }}}.
+Proof.
+Admitted.
+
+Lemma wp_MemKVCoordServer__Start (s:loc) (host : u64) γ :
+handlers_dom host γ.(coord_urpc_gn) {[ U64 1; U64 2 ]} -∗
+is_coord_server host γ -∗
+is_MemKVCoordServer s γ -∗
+  {{{
+       True
+  }}}
+    MemKVCoord__Start #s #host
+  {{{
+       RET #(); True
+  }}}.
+Proof.
+  iIntros "#Hdom #His_coord #His_memkv !#" (Φ) "_ HΦ".
+  wp_lam.
+  wp_pures.
+  change (Alloc (InjLV (λ: <>, (λ: <>, #())%V))) with
+      (NewMap ((slice.T byteT -> refT (slice.T byteT) -> unitT)%ht)).
+  wp_apply map.wp_NewMap.
+  iIntros (handlers_ptr) "Hmap".
+  wp_pures.
+
+  wp_apply (map.wp_MapInsert with "Hmap").
+  iIntros "Hmap".
+  wp_pures.
+  rewrite /MemKVCoord__GetShardMapRPC.
+
+  wp_apply (map.wp_MapInsert with "Hmap").
+  iIntros "Hmap".
+  wp_pures.
+
+  wp_apply (wp_MakeRPCServer with "[$Hmap]").
+  iIntros (rs) "Hsown".
+  wp_pures.
+
+  iNamed "His_coord".
+  wp_apply (wp_StartRPCServer with "[$Hsown]").
+  { rewrite ?dom_insert_L; set_solver. }
+  {
+    iSplitL "".
+    { rewrite /handlers_complete.
+      rewrite ?dom_insert_L dom_empty_L. iExactEq "Hdom". f_equal. set_solver. }
+    iApply (big_sepM_insert_2 with "").
+    { (* GetShardMapping RPC handler_is *)
+      iExists _, _, _.
+      iFrame "#HgetSpec".
+
+      clear Φ.
+      iIntros (?????) "!#".
+      iIntros (Φ) "Hpre HΦ".
+      wp_pures.
+      iDestruct "Hpre" as "(Hreq_sl & Hrep & _)".
+      simpl.
+      iNamed "His_memkv".
+      wp_loadField.
+      wp_apply (acquire_spec with "[$HmuInv]").
+      iIntros "[Hlocked Hown]".
+      iNamed "Hown".
+      wp_pures.
+      wp_apply (wp_struct_fieldRef_mapsto with "[$shardMap]").
+      { eauto. }
+      iIntros (fl) "(H1&H2)".
+      wp_apply (wp_encodeShardMap with "[$]").
+      iIntros (sl data) "(%Henc&H)".
+      wp_apply (wp_StoreAt with "[$]").
+      { apply slice_val_ty. }
+      iIntros "Hrep".
+      iNamed "H".
+      wp_pures.
+      wp_loadField.
+      wp_apply (release_spec with "[-HΦ Hrep Hdata]").
+      { iFrame "Hlocked HmuInv".
+        iNext. iExists _, _, _, _, _, _. iFrame. iFrame "#". iFrame "%".
+        iDestruct "H1" as %Hequiv. iApply Hequiv. iFrame. }
+      iApply "HΦ". iFrame. iNext. iExists _. iFrame "% #".
+    }
+    iApply (big_sepM_insert_2 with "").
+    { (* AddServerRPC *)
+      iExists _, _, _.
+      iFrame "#HaddSpec".
+
+      clear Φ.
+      iIntros (?????) "!#".
+      iIntros (Φ) "Hpre HΦ".
+      wp_pures.
+      iDestruct "Hpre" as "(Hreq_sl & Hrep & Hpre)".
+      simpl.
+      iDestruct "Hpre" as "(%Henc&Hshard)".
+      iDestruct "Hshard" as (γsh Heq) "#His_shard".
+      wp_apply (wp_decodeUint64 with "[$Hreq_sl]"); first eauto.
+      wp_pures.
+      simpl in x.
+      wp_apply (wp_MemKVCoord__AddServerRPC with "[Hrep]").
+      { iSplitL "". 
+        { rewrite /named. iExactEq "His_memkv". eauto. }
+        iFrame "His_shard". eauto.
+      }
+      iIntros (??) "(H1&H2)". iApply ("HΦ" with "[$H1 $H2]"); eauto.
+    }
+    rewrite big_sepM_empty. eauto.
+  }
+  iApply "HΦ".
+  auto.
+Qed.
+
+End memkv_coord_start_proof.
